Cross compiled to python

bin/RoundRobinScheduler-py/module_.py
@@ -1,0 +1,297 @@
+import sys
+from typing import Callable, Any, TypeVar, NamedTuple
+from math import floor
+from itertools import count
+
+import module_ as module_
+import _dafny as _dafny
+import System_ as System_
+
+# Module: module_
+
+class default__:
+    def  __init__(self):
+        pass
+
+    @staticmethod
+    def UniqueSeqLengthAtMostN(s, n):
+        d_0_numbersSet_: _dafny.Set
+        d_0_numbersSet_ = _dafny.Set({})
+        d_1_i_: int
+        d_1_i_ = 0
+        while (d_1_i_) < (n):
+            d_0_numbersSet_ = (d_0_numbersSet_) | (_dafny.Set({d_1_i_}))
+            d_1_i_ = (d_1_i_) + (1)
+        d_2_sSet_: _dafny.Set
+        d_2_sSet_ = _dafny.Set({})
+        d_3_j_: int
+        d_3_j_ = 0
+        while (d_3_j_) < (len(s)):
+            d_2_sSet_ = (d_2_sSet_) | (_dafny.Set({(s)[d_3_j_]}))
+            d_3_j_ = (d_3_j_) + (1)
+
+    @staticmethod
+    def SetOfIntegers(n):
+        def iife0_():
+            coll0_ = _dafny.Set()
+            compr_0_: int
+            for compr_0_ in _dafny.IntegerRange(0, n):
+                d_0_i_: int = compr_0_
+                if ((0) <= (d_0_i_)) and ((d_0_i_) < (n)):
+                    coll0_ = coll0_.union(_dafny.Set([d_0_i_]))
+            return _dafny.Set(coll0_)
+        return iife0_()
+        
+
+    @staticmethod
+    def ProcessQueueCurTime(processes, currentTime):
+        def lambda0_(forall_var_0_):
+            d_0_p_: Process = forall_var_0_
+            return not ((d_0_p_) in (_dafny.SeqWithoutIsStrInference((processes)[::]))) or ((((d_0_p_.inQueue) == (True)) or ((d_0_p_.isComplete) == (True)) if (d_0_p_.arrivalTime) <= (currentTime) else ((d_0_p_.inQueue) == (False)) or ((d_0_p_.isComplete) == (False))))
+
+        return _dafny.quantifier((_dafny.SeqWithoutIsStrInference((processes)[::])).UniqueElements, True, lambda0_)
+
+    @staticmethod
+    def AllPinProcessQueue(processes):
+        def lambda0_(forall_var_0_):
+            d_0_p_: Process = forall_var_0_
+            return not ((d_0_p_) in (_dafny.SeqWithoutIsStrInference((processes)[::]))) or (not(((d_0_p_.inQueue) == (True)) and ((d_0_p_.isComplete) == (True))))
+
+        return _dafny.quantifier((_dafny.SeqWithoutIsStrInference((processes)[::])).UniqueElements, True, lambda0_)
+
+    @staticmethod
+    def CheckForNewArrivals(processes, n, currentTime, readyQueue, extraInQueue):
+        newQueue: _dafny.Seq = _dafny.Seq({})
+        d_0_i_: int
+        d_0_i_ = 0
+        newQueue = readyQueue
+        d_1_added_: bool
+        d_1_added_ = False
+        while (d_0_i_) < (n):
+            if ((((processes)[d_0_i_].arrivalTime) <= (currentTime)) and (not((processes)[d_0_i_].inQueue))) and (not((processes)[d_0_i_].isComplete)):
+                obj0_ = (processes)[d_0_i_]
+                obj0_.inQueue = True
+                newQueue = (newQueue) + (_dafny.SeqWithoutIsStrInference([d_0_i_]))
+                d_1_added_ = True
+            default__.UniqueSeqLengthAtMostN(newQueue, n)
+            d_2_newSet_: _dafny.Set
+            def iife0_():
+                coll0_ = _dafny.Set()
+                compr_0_: int
+                for compr_0_ in _dafny.IntegerRange(0, n):
+                    d_3_i_: int = compr_0_
+                    if ((((0) <= (d_3_i_)) and ((d_3_i_) < (n))) and (((processes)[d_3_i_].isComplete) == (True))) and (((processes)[d_3_i_].inQueue) == (False)):
+                        coll0_ = coll0_.union(_dafny.Set([d_3_i_]))
+                return _dafny.Set(coll0_)
+            d_2_newSet_ = iife0_()
+            
+            d_0_i_ = (d_0_i_) + (1)
+        return newQueue
+
+    @staticmethod
+    def UpdateQueue(processes, n, quantum, readyQueue, currentTime, programsExecuted):
+        newQueue: _dafny.Seq = _dafny.Seq({})
+        updatedTime: int = int(0)
+        updatedExecuted: int = int(0)
+        updatedTime = currentTime
+        updatedExecuted = programsExecuted
+        d_0_i_: int
+        d_0_i_ = (readyQueue)[0]
+        newQueue = _dafny.SeqWithoutIsStrInference((readyQueue)[1::])
+        if ((processes)[d_0_i_].burstTimeRemaining) <= (quantum):
+            d_1_count_: _dafny.Set
+            def iife0_():
+                coll0_ = _dafny.Set()
+                compr_0_: int
+                for compr_0_ in _dafny.IntegerRange(0, n):
+                    d_2_i_: int = compr_0_
+                    if ((((0) <= (d_2_i_)) and ((d_2_i_) < (n))) and (((processes)[d_2_i_].isComplete) == (True))) and (((processes)[d_2_i_].inQueue) == (False)):
+                        coll0_ = coll0_.union(_dafny.Set([d_2_i_]))
+                return _dafny.Set(coll0_)
+            d_1_count_ = iife0_()
+            
+            obj0_ = (processes)[d_0_i_]
+            obj0_.inQueue = False
+            obj1_ = (processes)[d_0_i_]
+            obj1_.isComplete = True
+            updatedTime = (currentTime) + ((processes)[d_0_i_].burstTimeRemaining)
+            obj2_ = (processes)[d_0_i_]
+            obj2_.completionTime = updatedTime
+            obj3_ = (processes)[d_0_i_]
+            obj3_.waitingTime = (((processes)[d_0_i_].completionTime) - ((processes)[d_0_i_].arrivalTime)) - ((processes)[d_0_i_].burstTime)
+            if ((processes)[d_0_i_].waitingTime) < (0):
+                obj4_ = (processes)[d_0_i_]
+                obj4_.waitingTime = 0
+            obj5_ = (processes)[d_0_i_]
+            obj5_.turnaroundTime = ((processes)[d_0_i_].waitingTime) + ((processes)[d_0_i_].burstTime)
+            obj6_ = (processes)[d_0_i_]
+            obj6_.burstTimeRemaining = 0
+            d_3_newcount_: _dafny.Set
+            def iife1_():
+                coll1_ = _dafny.Set()
+                compr_1_: int
+                for compr_1_ in _dafny.IntegerRange(0, n):
+                    d_4_i_: int = compr_1_
+                    if ((((0) <= (d_4_i_)) and ((d_4_i_) < (n))) and (((processes)[d_4_i_].isComplete) == (True))) and (((processes)[d_4_i_].inQueue) == (False)):
+                        coll1_ = coll1_.union(_dafny.Set([d_4_i_]))
+                return _dafny.Set(coll1_)
+            d_3_newcount_ = iife1_()
+            
+            updatedExecuted = (programsExecuted) + (1)
+            if (updatedExecuted) != (n):
+                out0_: _dafny.Seq
+                out0_ = default__.CheckForNewArrivals(processes, n, updatedTime, newQueue, False)
+                newQueue = out0_
+            elif True:
+                pass
+        elif True:
+            d_5_count_: _dafny.Set
+            def iife2_():
+                coll2_ = _dafny.Set()
+                compr_2_: int
+                for compr_2_ in _dafny.IntegerRange(0, n):
+                    d_6_i_: int = compr_2_
+                    if ((((0) <= (d_6_i_)) and ((d_6_i_) < (n))) and (((processes)[d_6_i_].isComplete) == (True))) and (((processes)[d_6_i_].inQueue) == (False)):
+                        coll2_ = coll2_.union(_dafny.Set([d_6_i_]))
+                return _dafny.Set(coll2_)
+            d_5_count_ = iife2_()
+            
+            obj7_ = (processes)[d_0_i_]
+            obj7_.burstTimeRemaining = ((processes)[d_0_i_].burstTimeRemaining) - (quantum)
+            updatedTime = (currentTime) + (quantum)
+            newQueue = (newQueue) + (_dafny.SeqWithoutIsStrInference([d_0_i_]))
+            out1_: _dafny.Seq
+            out1_ = default__.CheckForNewArrivals(processes, n, updatedTime, newQueue, True)
+            newQueue = out1_
+        return newQueue, updatedTime, updatedExecuted
+
+    @staticmethod
+    def SeqProcSum(ps):
+        if (len(ps)) == (0):
+            return 0
+        elif True:
+            return ((default__.SeqProcSum(_dafny.SeqWithoutIsStrInference((ps)[:(len(ps)) - (1):]))) + ((ps)[(len(ps)) - (1)].arrivalTime)) + ((ps)[(len(ps)) - (1)].burstTime)
+
+    @staticmethod
+    def SumProcessTimes(ps):
+        total: int = int(0)
+        d_0_i_: int
+        d_0_i_ = 0
+        total = 0
+        while (d_0_i_) < (len(ps)):
+            total = ((total) + ((ps)[d_0_i_].arrivalTime)) + ((ps)[d_0_i_].burstTime)
+            d_0_i_ = (d_0_i_) + (1)
+        return total
+
+    @staticmethod
+    def RoundRobin(processes, n, quantum):
+        programsExecuted: int = int(0)
+        d_0_readyQueue_: _dafny.Seq
+        d_0_readyQueue_ = _dafny.SeqWithoutIsStrInference([0])
+        d_1_currentTime_: int
+        d_1_currentTime_ = 0
+        obj0_ = (processes)[0]
+        obj0_.inQueue = True
+        hi0_ = n
+        for d_2_i_ in range(1, hi0_):
+            if ((processes)[d_2_i_].arrivalTime) <= (d_1_currentTime_):
+                obj1_ = (processes)[d_2_i_]
+                obj1_.inQueue = True
+                d_0_readyQueue_ = (d_0_readyQueue_) + (_dafny.SeqWithoutIsStrInference([d_2_i_]))
+        default__.UniqueSeqLengthAtMostN(d_0_readyQueue_, n)
+        programsExecuted = 0
+        d_3_maxTime_: int
+        out0_: int
+        out0_ = default__.SumProcessTimes(processes)
+        d_3_maxTime_ = out0_
+        while ((programsExecuted) < (n)) and ((d_1_currentTime_) < (d_3_maxTime_)):
+            d_4_newQueue_: _dafny.Seq = _dafny.Seq({})
+            d_5_updatedTime_: int = int(0)
+            d_6_updatedExecuted_: int = int(0)
+            out1_: _dafny.Seq
+            out2_: int
+            out3_: int
+            out1_, out2_, out3_ = default__.UpdateQueue(processes, n, quantum, d_0_readyQueue_, d_1_currentTime_, programsExecuted)
+            d_4_newQueue_ = out1_
+            d_5_updatedTime_ = out2_
+            d_6_updatedExecuted_ = out3_
+            d_0_readyQueue_ = d_4_newQueue_
+            d_1_currentTime_ = d_5_updatedTime_
+            programsExecuted = d_6_updatedExecuted_
+        d_7_completedNotInQueue_: _dafny.Set
+        def iife0_():
+            coll0_ = _dafny.Set()
+            compr_0_: int
+            for compr_0_ in _dafny.IntegerRange(0, n):
+                d_8_i_: int = compr_0_
+                if ((((0) <= (d_8_i_)) and ((d_8_i_) < (n))) and (((processes)[d_8_i_].isComplete) == (True))) and (((processes)[d_8_i_].inQueue) == (False)):
+                    coll0_ = coll0_.union(_dafny.Set([d_8_i_]))
+            return _dafny.Set(coll0_)
+        d_7_completedNotInQueue_ = iife0_()
+        
+        return programsExecuted
+
+    @staticmethod
+    def Main(noArgsParameter__):
+        userInput = input("Enter number of processes: ")
+        d_0_n_: int
+        d_0_n_ = 4
+        d_1_quantum_: int
+        d_1_quantum_ = 1
+        d_2_processes_: _dafny.Seq
+        d_2_processes_ = _dafny.SeqWithoutIsStrInference([])
+        d_3_temp_: Process
+        nw0_ = Process()
+        nw0_.ctor__(1, 0, 5)
+        d_3_temp_ = nw0_
+        d_2_processes_ = (d_2_processes_) + (_dafny.SeqWithoutIsStrInference([d_3_temp_]))
+        nw1_ = Process()
+        nw1_.ctor__(2, 1, 3)
+        d_3_temp_ = nw1_
+        d_2_processes_ = (d_2_processes_) + (_dafny.SeqWithoutIsStrInference([d_3_temp_]))
+        nw2_ = Process()
+        nw2_.ctor__(3, 2, 8)
+        d_3_temp_ = nw2_
+        d_2_processes_ = (d_2_processes_) + (_dafny.SeqWithoutIsStrInference([d_3_temp_]))
+        nw3_ = Process()
+        nw3_.ctor__(4, 3, 6)
+        d_3_temp_ = nw3_
+        d_2_processes_ = (d_2_processes_) + (_dafny.SeqWithoutIsStrInference([d_3_temp_]))
+        d_4_completed_: int
+        out0_: int
+        out0_ = default__.RoundRobin(d_2_processes_, d_0_n_, d_1_quantum_)
+        d_4_completed_ = out0_
+        default__.printOutput(d_2_processes_)
+    
+    @staticmethod
+    def printOutput(processes):
+        for p in processes:
+            print(f"Process ID: {p.pid}, Arrival: {p.arrivalTime}, Burst Time: {p.burstTime}, Burst Time Remaining: {p.burstTimeRemaining}, Completion Time: {p.completionTime}, Turn Around Time: {p.turnaroundTime}, Waiting Time: {p.waitingTime}, In Queue: {p.inQueue}, Completed? {p.isComplete}")
+
+
+class Process:
+    def  __init__(self):
+        self.pid: int = int(0)
+        self.arrivalTime: int = int(0)
+        self.burstTime: int = int(0)
+        self.burstTimeRemaining: int = int(0)
+        self.completionTime: int = int(0)
+        self.turnaroundTime: int = int(0)
+        self.waitingTime: int = int(0)
+        self.isComplete: bool = False
+        self.inQueue: bool = False
+        pass
+
+    def __dafnystr__(self) -> str:
+        return "_module.Process"
+    def ctor__(self, id, arrival, burst):
+        (self).pid = id
+        (self).arrivalTime = arrival
+        (self).burstTime = burst
+        (self).burstTimeRemaining = burst
+        (self).completionTime = 0
+        (self).turnaroundTime = 0
+        (self).waitingTime = 0
+        (self).isComplete = False
+        (self).inQueue = False
+
